refactor: aimless meandering

Lean4Lean/Theory/Typing/Stratified.lean
@@ -22,11 +22,11 @@ nonrec theorem DefInv.symm (h : DefInv env U Γ e1 e2) : DefInv env U Γ e2 e1 :
 section
 set_option hygiene false
 local notation:65 Γ " ⊢ " e " : " A:30 => HasType1 Γ e A
-local notation:65 Γ " ⊢ " e1 " ≡ " e2:30 => IsDefEq1 Γ e1 e2
+local notation:65 Γ " ⊢ " e1 " ≡ " e2 " : " A:30 => IsDefEq1 Γ e1 e2 A
 
 variable (env : VEnv) (uvars : Nat)
 
-variable (IsDefEq1 : List VExpr → VExpr → VExpr → Prop) in
+variable (IsDefEq1 : List VExpr → VExpr → VExpr → VExpr → Prop) in
 inductive HasType1 : List VExpr → VExpr → VExpr → Prop where
   | bvar : Lookup Γ i A → Γ ⊢ .bvar i : A
   | const :
@@ -38,42 +38,42 @@ inductive HasType1 : List VExpr → VExpr → VExpr → Prop where
   | app : Γ ⊢ f : .forallE A B → Γ ⊢ a : A → Γ ⊢ .app f a : B.inst a
   | lam : Γ ⊢ A : .sort u → A::Γ ⊢ body : B → Γ ⊢ .lam A body : .forallE A B
   | forallE : Γ ⊢ A : .sort u → A::Γ ⊢ body : .sort v → Γ ⊢ .forallE A body : .sort (.imax u v)
-  | defeq : Γ ⊢ A ≡ B → Γ ⊢ e : A → Γ ⊢ e : B
-  | inst : A::Γ ⊢ e : B → Γ ⊢ e' : A → Γ ⊢ e.inst e' : B.inst e'
+  | defeq : Γ ⊢ A ≡ B : .sort u → Γ ⊢ e : A → Γ ⊢ e : B
 
-variable (HasType1 : List VExpr → VExpr → VExpr → Prop) in
-inductive IsDefEq1 : List VExpr → VExpr → VExpr → Prop where
-  | refl : Γ ⊢ e : A → Γ ⊢ e ≡ e
-  | symm : Γ ⊢ e ≡ e' → Γ ⊢ e' ≡ e
-  | trans : Γ ⊢ e₁ ≡ e₂ → Γ ⊢ e₂ ≡ e₃ → Γ ⊢ e₁ ≡ e₃
-  | sortDF : l.WF uvars → l'.WF uvars → l ≈ l' → Γ ⊢ .sort l ≡ .sort l'
+variable
+  (HasType1 : List VExpr → VExpr → VExpr → Prop)
+  (defEq : List VExpr → VExpr → VExpr → VExpr → Prop) in
+inductive IsDefEq1 : List VExpr → VExpr → VExpr → VExpr → Prop where
+  | refl : Γ ⊢ e : A → Γ ⊢ e ≡ e : A
+  | symm : Γ ⊢ e ≡ e' : A → Γ ⊢ e' ≡ e : A
+  | trans : Γ ⊢ e₁ ≡ e₂ : A → Γ ⊢ e₂ ≡ e₃ : A → Γ ⊢ e₁ ≡ e₃ : A
+  | sortDF : l.WF uvars → l'.WF uvars → l ≈ l' → Γ ⊢ .sort l ≡ .sort l' : .sort l.succ
   | appDF :
-    Γ ⊢ f : .forallE A B → Γ ⊢ f' : .forallE A B → Γ ⊢ a : A → Γ ⊢ a' : A →
-    Γ ⊢ f ≡ f' → Γ ⊢ a ≡ a' → Γ ⊢ .app f a ≡ .app f' a'
-  | lamDF : Γ ⊢ A ≡ A' → A::Γ ⊢ B ≡ B' → Γ ⊢ .lam A B ≡ .lam A' B'
-  | forallEDF : Γ ⊢ A ≡ A' → A::Γ ⊢ B ≡ B' → Γ ⊢ .forallE A B ≡ .forallE A' B'
-  | instDF :
-    A::Γ ⊢ f : B → A::Γ ⊢ f' : B → Γ ⊢ a : A → Γ ⊢ a' : A →
-    Γ ⊢ f ≡ f' → Γ ⊢ a ≡ a' → Γ ⊢ .inst f a ≡ .inst f' a'
-  | beta : A::Γ ⊢ e : B → Γ ⊢ e' : A → Γ ⊢ .app (.lam A e) e' ≡ e.inst e'
-  | eta : Γ ⊢ e : .forallE A B → Γ ⊢ .lam A (.app e.lift (.bvar 0)) ≡ e
-  | proofIrrel : Γ ⊢ p : .sort .zero → Γ ⊢ h : p → Γ ⊢ h' : p → Γ ⊢ h ≡ h'
+    Γ ⊢ f ≡ f' : .forallE A B → Γ ⊢ a ≡ a' : A → Γ ⊢ .app f a ≡ .app f' a' : B.inst a
+  | lamDF : Γ ⊢ A ≡ A' : .sort u → A::Γ ⊢ b ≡ b' : B → Γ ⊢ .lam A b ≡ .lam A' b' : .forallE A B
+  | forallEDF :
+    Γ ⊢ A ≡ A' : .sort u → A::Γ ⊢ B ≡ B' : .sort v →
+    Γ ⊢ .forallE A B ≡ .forallE A' B' : .sort (.imax u v)
+  | defeqDF : defEq Γ A B (.sort u) → Γ ⊢ e₁ ≡ e₂ : A → Γ ⊢ e₁ ≡ e₂ : B
+  | beta : A::Γ ⊢ e : B → Γ ⊢ e' : A → Γ ⊢ .app (.lam A e) e' ≡ e.inst e' : B.inst e'
+  | eta : Γ ⊢ e : .forallE A B → Γ ⊢ .lam A (.app e.lift (.bvar 0)) ≡ e : .forallE A B
+  | proofIrrel : Γ ⊢ p : .sort .zero → Γ ⊢ h : p → Γ ⊢ h' : p → Γ ⊢ h ≡ h' : p
   | extra :
     env.defeqs df → (∀ l ∈ ls, l.WF uvars) → ls.length = df.uvars →
-    Γ ⊢ df.lhs.instL ls ≡ df.rhs.instL ls
+    Γ ⊢ df.lhs.instL ls ≡ df.rhs.instL ls : df.type.instL ls
 
 end
 
 variable (henv : Ordered env) (hΓ : OnCtx Γ (env.IsType U)) in
 theorem IsDefEq.induction1
-    (defEq : List VExpr → VExpr → VExpr → Prop)
+    (defEq : List VExpr → VExpr → VExpr → VExpr → Prop)
     (hasType : List VExpr → VExpr → VExpr → Prop)
     (hty : ∀ {Γ e A}, HasType1 env U defEq Γ e A → hasType Γ e A)
-    (hdf : ∀ {Γ e1 e2}, IsDefEq1 env U hasType Γ e1 e2 → defEq Γ e1 e2)
+    (hdf : ∀ {Γ e1 e2 A}, IsDefEq1 env U hasType defEq Γ e1 e2 A → defEq Γ e1 e2 A)
     (H : env.IsDefEq U Γ e1 e2 A) :
     HasType1 env U defEq Γ e1 A ∧
     HasType1 env U defEq Γ e2 A ∧
-    IsDefEq1 env U hasType Γ e1 e2 := by
+    IsDefEq1 env U hasType defEq Γ e1 e2 A := by
   have H' := H.strong henv hΓ; clear hΓ H
   induction H' with
   | bvar h => exact ⟨.bvar h, .bvar h, .refl (hty (.bvar h))⟩
@@ -81,20 +81,19 @@ theorem IsDefEq.induction1
     exact ⟨.const h1 h2 h3, .const h1 h2 h3, .refl <| hty <| .const h1 h2 h3⟩
   | symm _ ih => exact ⟨ih.2.1, ih.1, .symm ih.2.2⟩
   | trans _ _ ih1 ih2 => exact ⟨ih1.1, ih2.2.1, .trans ih1.2.2 ih2.2.2⟩
-  | sortDF h1 h2 h3 =>
-    refine ⟨.sort h1, .defeq (hdf ?_) (.sort h2), .sortDF h1 h2 h3⟩
-    exact .symm <| .sortDF h1 h2 <| VLevel.succ_congr h3
+  | @sortDF l l' _ h1 h2 h3 =>
+    refine ⟨.sort h1, ?_, .sortDF h1 h2 h3⟩
+    exact .defeq (hdf <| .symm <| .sortDF (l' := l'.succ) h1 h2 (VLevel.succ_congr h3)) (.sort h2)
   | appDF _ _ _ _ _ _ _ _ _ ihf iha ihBa =>
     let ⟨hf, hf', ff⟩ := ihf; let ⟨ha, ha', aa⟩ := iha
-    exact ⟨.app hf ha, .defeq (hdf ihBa.2.2.symm) (.app hf' ha'),
-      .appDF (hty hf) (hty hf') (hty ha) (hty ha') ff aa⟩
+    exact ⟨.app hf ha, .defeq (hdf ihBa.2.2.symm) (.app hf' ha'), .appDF ff aa⟩
   | lamDF _ _ _ _ _ _ _ ihA ihB _ ihb ihb' =>
     refine ⟨.lam ihA.1 ihb.1, ?_, .lamDF ihA.2.2 ihb.2.2⟩
     exact .defeq (hdf <| .symm <| .forallEDF ihA.2.2 ihB.2.2) <| .lam ihA.2.1 ihb'.2.1
   | forallEDF _ _ _ _ _ ih1 ih2 ih3 =>
     exact ⟨.forallE ih1.1 ih2.1, .forallE ih1.2.1 ih3.2.1, .forallEDF ih1.2.2 ih2.2.2⟩
   | defeqDF _ _ _ ih1 ih2 =>
-    exact ⟨.defeq (hdf ih1.2.2) ih2.1, .defeq (hdf ih1.2.2) ih2.2.1, ih2.2.2⟩
+    exact ⟨.defeq (hdf ih1.2.2) ih2.1, .defeq (hdf ih1.2.2) ih2.2.1, .defeqDF (hdf ih1.2.2) ih2.2.2⟩
   | beta _ _ _ _ _ _ _ _ ihA _ ihe ihe' _ ihee =>
     exact ⟨.app (.lam ihA.1 ihe.1) ihe'.1, ihee.1, .beta (hty ihe.1) (hty ihe'.1)⟩
   | eta _ _ _ _ _ _ _ ihA _ _ ihe ihe' =>
@@ -105,6 +104,146 @@ theorem IsDefEq.induction1
     exact ⟨ih2.1, ih3.1, .proofIrrel (hty ih1.1) (hty ih2.1) (hty ih3.1)⟩
   | extra h1 h2 h3 _ _ _ _ _ _ _ _ _ ihl' ihr' =>
     exact ⟨ihl'.1, ihr'.1, .extra h1 h2 h3⟩
+
+variable (henv : Ordered env)
+  {defEq : List VExpr → VExpr → VExpr → VExpr → Prop}
+  (IH : ∀ {Γ e1 e2 A}, defEq Γ e1 e2 A → env.IsDefEq U Γ e1 e2 A) in
+theorem HasType1.induction (H : env.HasType1 U defEq Γ e A) : env.HasType U Γ e A := by
+  induction H with
+  | bvar h => exact .bvar h
+  | const h1 h2 h3 => exact .const h1 h2 h3
+  | sort h => exact .sort h
+  | app _ _ ih1 ih2 => exact .app ih1 ih2
+  | lam _ _ ih1 ih2 => exact .lam ih1 ih2
+  | forallE _ _ ih1 ih2 => exact .forallE ih1 ih2
+  | defeq h1 _ ih => exact (IH h1).defeq ih
+
+variable (henv : Ordered env)
+  {hasType : List VExpr → VExpr → VExpr → Prop}
+  {defEq : List VExpr → VExpr → VExpr → VExpr → Prop}
+  (hty : ∀ {Γ e A}, hasType Γ e A → env.HasType U Γ e A)
+  (hdf : ∀ {Γ e1 e2 A}, defEq Γ e1 e2 A → env.IsDefEq U Γ e1 e2 A) in
+theorem IsDefEq1.induction
+    (H : env.IsDefEq1 U hasType defEq Γ e1 e2 A) : env.IsDefEq U Γ e1 e2 A := by
+  induction H with
+  | refl h => exact hty h
+  | symm _ ih => exact ih.symm
+  | trans _ _ ih1 ih2 => exact ih1.trans ih2
+  | sortDF h1 h2 h3 => exact .sortDF h1 h2 h3
+  | appDF _ _ ih1 ih2 => exact .appDF ih1 ih2
+  | lamDF _ _ ih1 ih2 => exact .lamDF ih1 ih2
+  | forallEDF _ _ ih1 ih2 => exact .forallEDF ih1 ih2
+  | defeqDF h1 _ ih => exact .defeqDF (hdf h1) ih
+  | beta h1 h2 => exact .beta (hty h1) (hty h2)
+  | eta h => exact .eta (hty h)
+  | proofIrrel h1 h2 h3 => exact .proofIrrel (hty h1) (hty h2) (hty h3)
+  | extra h1 h2 h3 => exact .extra h1 h2 h3
+
+/-
+variable
+  {U : Nat}
+  (hasType : List VExpr → VExpr → VExpr → Prop)
+  (hasType' : List VExpr → VExpr → VExpr → Prop)
+  (defEq : List VExpr → VExpr → VExpr → VExpr → Prop)
+  (refl : ∀ {Γ e A}, hasType Γ e A → hasType' Γ e A)
+  (sort : ∀ {Γ l l'}, l.WF U → l'.WF U → l ≈ l' →
+    hasType' Γ (.sort l') (.sort l.succ))
+  (app : ∀ {Γ f a A B},
+    hasType' Γ f (.forallE A B) → hasType' Γ a A → hasType' Γ (.app f a) (B.inst a))
+in
+protected theorem IsDefEq1.hasType_ind
+    (H : IsDefEq1 env U hasType defEq Γ e1 e2 A) :
+    hasType' Γ e1 A ∧ hasType' Γ e2 A := by
+  induction H with
+  | refl h => exact ⟨refl h, refl h⟩
+  | symm _ ih => exact ih.symm
+  | trans _ _ ih1 ih2 => exact ⟨ih1.1, ih2.2⟩
+  | sortDF h1 h2 h3 => exact ⟨sort h1 h1 rfl, sort h1 h2 h3⟩
+  | appDF _ _ ih1 ih2 =>
+    exact ⟨app ih1.1 ih2.1, app _ _⟩
+  | lamDF _ _ ih1 ih2 => exact .lamDF ih1 ih2
+  | forallEDF _ _ ih1 ih2 => exact .forallEDF ih1 ih2
+  | defeqDF h1 _ ih => exact .defeqDF (hdf h1) ih
+  | beta h1 h2 => exact .beta (hty h1) (hty h2)
+  | eta h => exact .eta (hty h)
+  | proofIrrel h1 h2 h3 => exact .proofIrrel (hty h1) (hty h2) (hty h3)
+  | extra h1 h2 h3 => exact .extra h1 h2 h3
+
+variable
+  (hasType : List VExpr → VExpr → VExpr → Prop)
+  (defEq : List VExpr → VExpr → VExpr → VExpr → Prop) in
+inductive IsDefEqU1 : List VExpr → VExpr → VExpr → VLevel → Prop
+  | refl : hasType Γ A (.sort u) → IsDefEqU1 Γ A A u
+
+variable (henv : Ordered env)
+  {hasType : List VExpr → VExpr → VExpr → Prop}
+  {defEq : List VExpr → VExpr → VExpr → VExpr → Prop}
+  (refl : ∀ {Γ e A}, hasType Γ e A → defEq' Γ e e A)
+  (hdf : ∀ {Γ e1 e2 A}, defEq Γ e1 e2 A → env.IsDefEq U Γ e1 e2 A) in
+theorem IsDefEq1.unique_typing1
+    (H : env.IsDefEq1 U hasType defEq Γ e1 e2 A) :
+    hasType Γ e1 A ∧ hasType Γ e2 A := by
+  induction H with
+  | refl h => exact hty h
+  | symm _ ih => exact ih.symm
+  | trans _ _ ih1 ih2 => exact ih1.trans ih2
+  | sortDF h1 h2 h3 => exact .sortDF h1 h2 h3
+  | appDF _ _ ih1 ih2 => exact .appDF ih1 ih2
+  | lamDF _ _ ih1 ih2 => exact .lamDF ih1 ih2
+  | forallEDF _ _ ih1 ih2 => exact .forallEDF ih1 ih2
+  | defeqDF h1 _ ih => exact .defeqDF (hdf h1) ih
+  | beta h1 h2 => exact .beta (hty h1) (hty h2)
+  | eta h => exact .eta (hty h)
+  | proofIrrel h1 h2 h3 => exact .proofIrrel (hty h1) (hty h2) (hty h3)
+  | extra h1 h2 h3 => exact .extra h1 h2 h3
+
+variable (henv : Ordered env) in
+theorem HasType1.unique_typing'
+    (H1 : env.HasType1 U (IsDefEq1 env U hasType defEq) Γ e A1)
+    (H2 : env.HasType1 U (IsDefEq1 env U hasType defEq) Γ e A2) :
+    ∃ u, env.IsDefEq1 U hasType defEq Γ A1 A2 (.sort u) := by
+  generalize eq1 : e = e' at H2
+  induction H1 generalizing e' A2 with subst eq1
+  | defeq h1 _ ih =>
+    let ⟨_, ih⟩ := ih _ rfl H2
+    exact ⟨_, h1.trans _⟩
+    done
+  | _ => ?_
+  <;> cases H2
+
+  case bvar.bvar _ =>
+    done
+  case const.const _ _ _ =>
+    done
+  case sort.sort _ =>
+    done
+  case app.app _ _ _ _ =>
+    done
+  case lam.lam _ _ _ _ =>
+    done
+  case forallE.forallE _ _ _ _ =>
+    done
+  case defeq.defeq _ _ _ =>
+    done
+  _
+  -- | bvar h =>
+  --   refine .bvar h.instL
+  -- | @const _ _ ls' _ h1 h2 h3 =>
+  --   simp [instL, instL_instL]
+  --   exact .const h1 (by simp [h2, VLevel.WF.inst hls]) (by simp [h3])
+  -- | sort _ _ h3 =>
+  --   exact .sortDF (VLevel.WF.inst hls) (VLevel.WF.inst hls) (VLevel.inst_congr_l h3)
+  -- | app _ _ ih1 ih2 => exact instL_instN ▸ .appDF ih1 ih2
+  -- | lam _ _ ih1 ih2 => exact .lamDF ih1 ih2
+  -- | forallEDF _ _ ih1 ih2 => exact .forallEDF ih1 ih2
+  -- | defeqDF _ _ ih1 ih2 => exact .defeqDF ih1 ih2
+  -- | beta _ _ ih1 ih2 => simpa using .beta ih1 ih2
+  -- | eta _ ih => simpa [instL] using .eta ih
+  -- | proofIrrel _ _ _ ih1 ih2 ih3 => exact .proofIrrel ih1 ih2 ih3
+  -- | extra h1 h2 h3 =>
+  --   simp [instL, instL_instL]
+  --   exact .extra h1 (by simp [h2, VLevel.WF.inst hls]) (by simp [h3])
+-/
 
 /-
 variable (henv : Ordered env) in
